Proof up to ber_check_tags

src/Lib/BCT/Exec.v
@@ -4,8 +4,8 @@ Require Import ExtLib.Structures.Monad.
 Import MonadNotation.
 
 (* checks the tag, outputs consumed length and expected length *)
-Definition ber_check_tags (td : TYPE_descriptor) 
-           (ls : list byte) : option check_tag_r :=
+Definition ber_check_tags (td : TYPE_descriptor) (ls : list byte) : 
+  option check_tag_r :=
   match decoder_type td with
   | BOOLEAN_t => match ls with
                 | x1::x2::_ => if ((x1 == Byte.one) && (x2 == Byte.one))%byte
@@ -15,4 +15,14 @@ Definition ber_check_tags (td : TYPE_descriptor)
                 end
   | _ => None
   end.
-  
+
+Theorem ber_check_tags_bool_succ : forall td ls,
+    decoder_type td = BOOLEAN_t ->
+    ber_check_tags td ([Byte.one; Byte.one] ++ ls) = 
+    Some (mk_check_tag_rval 2 1).
+Proof.
+  intros.
+  unfold ber_check_tags.
+  rewrite H.
+  reflexivity.
+Qed.
