src/Lib/BCT/Vst.v
@@ -2,7 +2,6 @@ Require Import Core.Core Core.StructNormalizer
         VstLib ErrorWithWriter BCT.Exec.
 Require Import VST.floyd.proofauto.
 Require Import Clight.ber_decoder.
-Require Export VST.floyd.Funspec_old_Notation.
 
 Definition Vprog : varspecs. mk_varspecs prog. Defined.
 Instance CompSpecs : compspecs. make_compspecs prog. Defined.
@@ -14,36 +13,36 @@ Section Ber_check_tags.
 Definition ber_check_tags_spec : ident * funspec :=
   DECLARE _ber_check_tags
     WITH (* Codec context pointer *) 
-         sh_ctx : share, ctx_b : block, ctx_ofs : ptrofs, ctx : val,
+         ctx_p : val, ctx : val,
          (* Type Descriptor pointer *)
-         sh_td : share, td_b : block, td_ofs : ptrofs, td : TYPE_descriptor,
+         td_p : val, td : TYPE_descriptor,
          (* Struct context pointer *) 
-         sh_ctx_s : share, ctx_s_b : block, ctx_s_ofs : ptrofs, ctx_s : val,
+         ctx_s_p : val, ctx_s : val,
          (* Buffer pointer *)
-         sh_ptr : share, ptr_b : block, ptr_ofs : ptrofs, ptr : list byte,
+         buf_p : val, buf : list byte,
          (* pointer to the return struct dec_rval *)                        
-         sh_res : share, res_b : block, res_ofs : ptrofs,
-         size : Z, tag_mode : Z, last_tag_from : Z
-         (* sh_ll : share, ll_b : block, ll_ofs : ptrofs, ll : val,
-         sh_opt : share, opt_b : block, opt_ofs : ptrofs, opt : val *)
-
-    PRE [ __res OF (tptr (Tstruct _asn_dec_rval_s noattr)),
-         _opt_codec_ctx OF (tptr (Tstruct _asn_codec_ctx_s noattr)),
-         _td OF (tptr (Tstruct _asn_TYPE_descriptor_s noattr)),
-         _opt_ctx OF (tptr (Tstruct _asn_struct_ctx_s noattr)),
-         _ptr OF (tptr tvoid),
-         _size OF tuint,
-         _tag_mode OF tint,
-         _last_tag_form OF tint,
-         _last_length OF (tptr tint),
-         _opt_tlv_form OF (tptr tint)]
-    PROP ( )
-    LOCAL ()
-    SEP ()
+         res_p : val,
+         size : Z, tag_mode : Z, last_tag_from : Z,
+         ll_p : val, ll : Z, opt_tlv_form_p : val, opt_tlv_form : Z
+    PRE [tptr asn_dec_rval_s, tptr (Tstruct _asn_codec_ctx_s noattr),
+         tptr (Tstruct _asn_TYPE_descriptor_s noattr),
+         tptr (Tstruct _asn_struct_ctx_s noattr), 
+         tptr tvoid, tuint, tint, tint, tptr tint, tptr tint]
+      PROP ()
+      PARAMS (res_p; ctx_p; td_p; ctx_s_p; buf_p; Vint (Int.repr size);
+              Vint (Int.repr tag_mode); Vint (Int.repr last_tag_from);
+              ll_p; opt_tlv_form_p)
+      GLOBALS ()
+      SEP (data_at_ Tsh asn_dec_rval_s res_p)
     POST [tvoid]
       PROP ()
       LOCAL ()
-      SEP ().
+      SEP (data_at Tsh asn_dec_rval_s 
+                   (match ber_check_tags td buf with
+                    | Some v => construct_dec_rval (tag_consumed v) (tag_expected v)
+                    | None => construct_dec_rval 0 0 
+                    (* TODO set appropriate values for failure *)
+                    end) res_p).
 
 Definition Gprog := ltac:(with_library prog [ber_check_tags_spec]).
 
